[WIP] play with modalities in UnifLogic

theories/Staging/UnifLogic.v
@@ -50,6 +50,7 @@ From Katamaran Require Import
      (* Syntax.Formulas *)
      Syntax.Predicates
      .
+From iris Require bi.derived_connectives bi.interface proofmode.tactics.
 
 Declare Scope pred_scope.
 Delimit Scope pred_scope with P.
@@ -452,492 +453,69 @@ Module Pred
     End Eq.
     #[global] Arguments eqₚ_trans {T A _ w} s t u.
 
-    (* Lemma peq_ty_noconfusion {w : World} (t1 t2 : OTy w) : *)
-    (*   t1 =ₚ t2 ⊣⊢ₚ *)
-    (*   match t1 , t2 with *)
-    (*   | oty.evar  _      , _                => t1 =ₚ t2 *)
-    (*   | _                , oty.evar _       => t1 =ₚ t2 *)
-    (*   | oty.bool         , oty.bool         => ⊤ₚ *)
-    (*   | oty.func t11 t12 , oty.func t21 t22 => t11 =ₚ t21 /\ₚ t12 =ₚ t22 *)
-    (*   | _                , _                => ⊥ₚ *)
-    (*   end. *)
-    (* Proof. destruct t1, t2; crushPredEntails3. Qed. *)
-
-    (* Lemma eq_pair *)
-    (*   {AT BT : OType} {A B : Type} {instA : Inst AT A} {instB : Inst BT B} *)
-    (*   [w] (a1 a2 : AT w) (b1 b2 : BT w) : *)
-    (*   (a1,b1) =ₚ (a2,b2) ⊣⊢ₚ ((a1 =ₚ a2) /\ₚ (b1 =ₚ b2)). *)
-    (* Proof. *)
-    (*   pred_unfold. intros ι; cbn. split. *)
-    (*   - now injection 1. *)
-    (*   - intros []. now f_equal. *)
-    (* Qed. *)
-
-    Section Subst.
-
-      (* Lemma subst_eq {T : OType} {substT : Subst T} *)
-      (*   {A : Type} {instTA : Inst T A} {instSubstTA : InstSubst T A} *)
-      (*   {Θ : SUB} {w0 w1} (θ : Θ w0 w1) (t1 t2 : T w0) : *)
-      (*   subst (t1 =ₚ t2) θ ⊣⊢ₚ subst t1 θ =ₚ subst t2 θ. *)
-      (* Proof. *)
-      (*   pred_unfold. unfold subst, subst_pred. intros ι. *)
-      (*   now rewrite !inst_subst. *)
-      (* Qed. *)
-
-      (* Context {Θ : SUB}. *)
-
-      (* We could define a SubstLaws instance for the Pred type, but that's
-         requires functional extensionality. Instead, we provide similar
-         lemmas that use bientailment instead of Leibniz equality and thus
-         avoid functional extensionality. *)
-      (* Lemma subst_pred_refl `{lkReflΘ : LkRefl Θ} [w] (P : Pred w) : *)
-      (*   subst P refl ⊣⊢ₚ P. *)
-      (* Proof. crushPredEntails3. Qed. *)
-      (* Lemma subst_pred_trans `{lktransΘ : LkTrans Θ} *)
-      (*   {w0 w1 w2} (θ1 : Θ w0 w1) (θ2 : Θ w1 w2) (P : Pred w0) : *)
-      (*   subst P (θ1 ⊙ θ2) ⊣⊢ₚ subst (subst P θ1) θ2. *)
-      (* Proof. crushPredEntails3. Qed. *)
-      (* Lemma subst_and {w0 w1} (θ : Θ w0 w1) (P Q : Pred w0) : *)
-      (*   subst (P /\ₚ Q) θ ⊣⊢ₚ subst P θ /\ₚ subst Q θ. *)
-      (* Proof. crushPredEntails3. Qed. *)
-      (* Lemma subst_impl {w0 w1} (θ : Θ w0 w1) (P Q : Pred w0) : *)
-      (*   subst (P ->ₚ Q) θ ⊣⊢ₚ (subst P θ ->ₚ subst Q θ). *)
-      (* Proof. crushPredEntails3. Qed. *)
-      (* Lemma subst_wand {w0 w1} (θ : Θ w0 w1) (P Q : Pred w0) : *)
-      (*   subst (interface.bi_wand P Q) θ ⊣⊢ₚ interface.bi_wand (subst P θ) (subst Q θ). *)
-      (* Proof. crushPredEntails3. Qed. *)
-      (* Lemma subst_false {w0 w1} (θ : Θ w0 w1) : *)
-      (*   subst ⊥ₚ θ ⊣⊢ₚ ⊥ₚ. *)
-      (* Proof. crushPredEntails3. Qed. *)
-      (* Lemma subst_true {w0 w1} (θ : Θ w0 w1) : *)
-      (*   subst ⊤ₚ θ ⊣⊢ₚ ⊤ₚ. *)
-      (* Proof. crushPredEntails3. Qed. *)
-      (* Lemma subst_forall [A] [w0 w1] (θ : Θ w0 w1) (Q : A -> Pred w0) : *)
-      (*   subst (∀ₚ a : A, Q a) θ ⊣⊢ₚ (∀ₚ a : A, subst (Q a) θ). *)
-      (* Proof. crushPredEntails3. Qed. *)
-      (* Lemma subst_exists [A] [w0 w1] (θ : Θ w0 w1) (Q : A -> Pred w0) : *)
-      (*   subst (∃ₚ a : A, Q a) θ ⊣⊢ₚ (∃ₚ a : A, subst (Q a) θ). *)
-      (* Proof. crushPredEntails3. Qed. *)
-
-      (* Lemma subst_tpb {w0 w1} (θ : Θ w0 w1) G (e : Exp) (t : OTy w0) (ee : OExp w0) : *)
-      (*   subst (G |--ₚ e; t ~> ee) θ ⊣⊢ₚ *)
-      (*   subst G θ |--ₚ e; subst t θ ~> subst ee θ. *)
-      (* Proof. crushPredEntails3. Qed. *)
-
-    End Subst.
-
   End Lemmas.
 
-  (* Module Sub. *)
-  (*   Import iris.bi.interface iris.bi.derived_laws.bi. *)
-  (*   Import (hints) Par. *)
-  (*   Section WithSubstitution. *)
-  (*     Context {Θ : SUB}. *)
+  Section SubstMod.
+    Import ModalNotations.
+
+    Lemma acc_pathcond {w1 w2} (ω : w2 ⊒ w1) :
+      forall ι,  instprop (wco w1) ι -> instprop (wco w2) (inst (sub_acc ω) ι).
+    Proof.
+      intros.
+      rewrite <-instprop_subst.
+      now apply (ent_acc_sub ω ι H).
+    Qed.
+
+
+    (* update: one of these requires an assumption of the path condition... *)
+    Definition before {w1 w2} (ω : w2 ⊒ w1) : Pred w1 -> Pred w2 :=
+      fun Rpast ι => forall ιpast, inst (sub_acc ω) ιpast = ι -> Rpast ιpast.
+    Definition after {w1 w2} (ω : w2 ⊒ w1) : Pred w2 -> Pred w1 :=
+      fun Rfut ι => Rfut (inst (sub_acc ω) ι).
+  End SubstMod.
+
+  Section LogicalRelation.
+    Import logicalrelation.
+    Import ModalNotations.
+    
+    Definition Related {AT A} (R : Rel AT A) : ⊢ AT -> Const A -> Pred :=
+      fun w t v ι => (instprop (wco w) ι -> RSat R ι t v)%type.
+
+  End LogicalRelation.
+
+  Module Import ufl_notations.
+    Import logicalrelation.
+    Open Scope rel_scope.
+    Notation "ℛ⟦ R ⟧" := (Related R%R) (format "ℛ⟦ R ⟧").
+    Notation "A -> B" := (RImpl A%R B%R) : rel_scope.
+    Notation "□ᵣ A"    := (RBox A%R) (at level 9) : rel_scope.
+    Notation "'∀ᵣ' x .. y , R " :=
+      (RForall (fun x => .. (RForall (fun y => R)) ..))
+        (at level 200, x binder, y binder, right associativity,
+          format "'[  ' '[  ' ∀ᵣ  x  ..  y ']' ,  '/' R ']'")
+        : rel_scope.
+  End ufl_notations.
+
+  Section LRCompat.
+    Import notations.
+    Import ufl_notations.
+    Import logicalrelation.
+    (* Import ModalNotations. *)
+    Import iris.proofmode.tactics.
+    
+
+    Lemma refine_four {w1 w2} {ω : Acc w2 w1} {AT A} (RA : Rel AT A) :
+      (⊢ ∀ (v__s : Box AT w2) v, (after ω (ℛ⟦□ᵣ RA⟧ w2 v__s v) ->ₚ ℛ⟦RBox RA⟧ w1 (four v__s ω) v))%P.
+    Proof.
+      constructor.
+      intros ι2 Hpc _ _ v__s _ v _ Htv _ w0 r01 ι0 -> Hpc0.
+      unfold four, after in *.
+      unfold RBox, Related in Htv. cbn in Htv.
+      apply Htv.
+      - now apply acc_pathcond.
+      - now rewrite <-inst_subst, sub_acc_trans.
+      - done.
+    Qed.
 
-  (*     Definition wp {w0 w1} (θ : Θ w0 w1) (Q : Pred w1) : Pred w0 := *)
-  (*       fun ι0 => exists (ι1 : Assignment w1), inst θ ι1 = ι0 /\ Q ι1. *)
-  (*     Definition wlp {w0 w1} (θ : Θ w0 w1) (Q : Pred w1) : Pred w0 := *)
-  (*       fun ι0 => forall (ι1 : Assignment w1), inst θ ι1 = ι0 -> Q ι1. *)
-
-  (*     #[global] Arguments wp {_ _} _ _ ι0/. *)
-  (*     #[global] Arguments wlp {_ _} _ _ ι0/. *)
-
-  (*     #[export] Instance proper_wp_bientails {w0 w1} (θ : Θ w0 w1) : *)
-  (*       Proper ((⊣⊢ₚ) ==> (⊣⊢ₚ)) (wp θ). *)
-  (*     Proof. firstorder. Qed. *)
-
-  (*     #[export] Instance proper_wp_entails {w0 w1} (θ : Θ w0 w1) : *)
-  (*       Proper ((⊢ₚ) ==> (⊢ₚ)) (wp θ). *)
-  (*     Proof. firstorder. Qed. *)
-
-  (*     #[export] Instance proper_wlp_bientails {w0 w1} (θ : Θ w0 w1) : *)
-  (*       Proper ((⊣⊢ₚ) ==> (⊣⊢ₚ)) (wlp θ). *)
-  (*     Proof. firstorder. Qed. *)
-
-  (*     #[export] Instance proper_wlp_entails {w0 w1} (θ : Θ w0 w1) : *)
-  (*       Proper ((⊢ₚ) ==> (⊢ₚ)) (wlp θ). *)
-  (*     Proof. firstorder. Qed. *)
-
-  (*     Lemma wp_refl {reflΘ : Refl Θ} {lkreflΘ : LkRefl Θ} *)
-  (*       {w} (Q : Pred w) : wp refl Q ⊣⊢ₚ Q. *)
-  (*     Proof. *)
-  (*       unfold wp; pred_unfold. intros ι; split. *)
-  (*       - intros (ι' & Heq & HQ). now subst. *)
-  (*       - intros HQ. exists ι. easy. *)
-  (*     Qed. *)
-
-  (*     Lemma wp_trans {transR : Trans Θ} {lktransΘ : LkTrans Θ} *)
-  (*       {w0 w1 w2} (θ1 : Θ w0 w1) (θ2 : Θ w1 w2) Q : *)
-  (*       wp (θ1 ⊙ θ2) Q ⊣⊢ₚ wp θ1 (wp θ2 Q). *)
-  (*     Proof. *)
-  (*       unfold wp; pred_unfold. intros ι; split. *)
-  (*       - intros (ι2 & Heq & HQ). eauto. *)
-  (*       - intros (ι1 & Heq1 & ι2 & Heq2 & HQ). subst. eauto. *)
-  (*     Qed. *)
-
-  (*     Lemma wp_false {w0 w1} (θ : Θ w0 w1) : *)
-  (*       wp θ ⊥ₚ ⊣⊢ₚ ⊥ₚ. *)
-  (*     Proof. firstorder. Qed. *)
-
-  (*     Lemma and_wp_l {w0 w1} (θ : Θ w0 w1) P Q : *)
-  (*       wp θ P /\ₚ Q ⊣⊢ₚ wp θ (P /\ₚ subst Q θ). *)
-  (*     Proof. *)
-  (*       unfold wp; pred_unfold. split. *)
-  (*       - intros [(ι1 & <- & HP) HQ]. eauto. *)
-  (*       - intros (ι1 & <- & HP & HQ). eauto. *)
-  (*     Qed. *)
-
-  (*     Lemma and_wp_r {w0 w1} (θ : Θ w0 w1) (P : Pred w0) (Q : Pred w1) : *)
-  (*       P /\ₚ wp θ Q ⊣⊢ₚ wp θ (subst P θ /\ₚ Q). *)
-  (*     Proof. now rewrite and_comm and_wp_l and_comm. Qed. *)
-
-  (*     Lemma wp_thick {thickΘ : Thick Θ} {lkThickΘ : LkThick Θ} *)
-  (*       {w α} (αIn : world.In α w) (t : OTy (w - α)) (Q : Pred (w - α)) : *)
-  (*       wp (thick α t) Q ⊣⊢ₚ oty.evar αIn =ₚ subst t (thin (Θ := Par) α) /\ₚ subst Q (thin (Θ := Par) α). *)
-  (*     Proof. *)
-  (*       unfold wp; pred_unfold. intros ι. split. *)
-  (*       - intros (ι1 & Heq & HQ). subst. *)
-  (*         now rewrite inst_thick env.remove_insert env.lookup_insert. *)
-  (*       - intros [Heq HQ]. exists (env.remove α ι αIn). *)
-  (*         now rewrite inst_thick -Heq env.insert_remove. *)
-  (*     Qed. *)
-
-  (*     Lemma wlp_refl {reflΘ : Refl Θ} {lkreflΘ : LkRefl Θ} *)
-  (*       {w} (Q : Pred w) : wlp refl Q ⊣⊢ₚ Q. *)
-  (*     Proof. *)
-  (*       unfold wlp; pred_unfold. intros ι. split. *)
-  (*       - intros HQ. auto. *)
-  (*       - intros HQ ? <-. auto. *)
-  (*     Qed. *)
-
-  (*     Lemma wlp_trans {transR : Trans Θ} {lktransΘ : LkTrans Θ} *)
-  (*       {w0 w1 w2} (θ1 : Θ w0 w1) (θ2 : Θ w1 w2) Q : *)
-  (*       wlp (θ1 ⊙ θ2) Q ⊣⊢ₚ wlp θ1 (wlp θ2 Q). *)
-  (*     Proof. *)
-  (*       unfold wlp; pred_unfold. intros ι. split. *)
-  (*       - intros HQ ι1 Heq1 ι2 Heq2. subst; auto. *)
-  (*       - intros HQ ι2 Heq. subst; eauto. *)
-  (*     Qed. *)
-
-  (*     Lemma wlp_true {w0 w1} (θ : Θ w0 w1) : *)
-  (*       wlp θ ⊤ₚ ⊣⊢ₚ ⊤ₚ. *)
-  (*     Proof. firstorder. Qed. *)
-
-  (*     (* Lemma wlp_and {w0 w1} (θ : Θ w0 w1) P Q : *) *)
-  (*     (*   wlp θ P /\ₚ wlp θ Q ⊣⊢ₚ wlp θ (P /\ₚ Q). *) *)
-  (*     (* Proof. firstorder. Qed. *) *)
-
-  (*     (* Lemma wp_or {w0 w1} (θ : Θ w0 w1) P Q : *) *)
-  (*     (*   wp θ P \/ₚ wp θ Q ⊣⊢ₚ wp θ (P \/ₚ Q). *) *)
-  (*     (* Proof. firstorder. Qed. *) *)
-
-  (*     Lemma wp_mono {w0 w1} (θ : Θ w0 w1) P Q: *)
-  (*       wlp θ (interface.bi_wand P Q) ⊢ₚ interface.bi_wand (wp θ P) (wp θ Q). *)
-  (*     Proof. firstorder. Qed. *)
-
-  (*     Lemma wlp_mono {w0 w1} (θ : Θ w0 w1) P Q : *)
-  (*       wlp θ (interface.bi_wand P Q) ⊢ₚ interface.bi_wand (wlp θ P) (wlp θ Q). *)
-  (*     Proof. firstorder. Qed. *)
-
-  (*     Lemma entails_wlp {w0 w1} (θ : Θ w0 w1) P Q : *)
-  (*       (subst P θ ⊢ₚ Q) <-> (P ⊢ₚ wlp θ Q). *)
-  (*     Proof. *)
-  (*       unfold wlp; pred_unfold. split; intros HPQ. *)
-  (*       - intros ι0 HP ι1 <-. revert HP. apply HPQ. *)
-  (*       - intros ι1 HP. now apply (HPQ (inst θ ι1)). *)
-  (*     Qed. *)
-
-  (*     Lemma entails_wp {w0 w1} (θ : Θ w0 w1) P Q : *)
-  (*       (P ⊢ₚ subst Q θ) <-> (wp θ P ⊢ₚ Q). *)
-  (*     Proof. *)
-  (*       unfold wp; pred_unfold. split; intros HPQ. *)
-  (*       - intros ι0 (ι1 & <- & HP). now apply HPQ. *)
-  (*       - intros ι1 HP. apply (HPQ (inst θ ι1)). exists ι1. split; auto. *)
-  (*     Qed. *)
-
-  (*     Lemma wp_impl {w0 w1} (θ1 : Θ w0 w1) (P : Pred _) (Q : Pred _) : *)
-  (*       (wp θ1 P ->ₚ Q) ⊣⊢ₚ wlp θ1 (P ->ₚ subst Q θ1). *)
-  (*     Proof. *)
-  (*       unfold wp, wlp; pred_unfold. intros ι0; split. *)
-  (*       - intros H ι1 <- HP. apply H. now exists ι1. *)
-  (*       - intros HPQ (ι1 & <- & HP). now apply HPQ. *)
-  (*     Qed. *)
-
-  (*     Lemma subst_wlp {w0 w1} {θ : Θ w0 w1} (P : Pred w1) : *)
-  (*       subst (wlp θ P) θ ⊢ₚ P. *)
-  (*     Proof. firstorder. Qed. *)
-
-  (*     (* Lemma subst_wp {w0 w1} {θ : Θ w0 w1} (P : Pred w1) : *) *)
-  (*     (*   P ⊢ₚ subst (wp θ P) θ. *) *)
-  (*     (* Proof. firstorder. Qed. *) *)
-
-  (*     Lemma wlp_frame {w0 w1} (θ : Θ w0 w1) (P : Pred _) (Q : Pred _) : *)
-  (*       P ->ₚ wlp θ Q ⊣⊢ₚ wlp θ (subst P θ ->ₚ Q). *)
-  (*     Proof. *)
-  (*       unfold wlp; pred_unfold. intros ι; split. *)
-  (*       - intros H ι1 <- HP. now apply (H HP). *)
-  (*       - intros H HP ι1 <-. apply H; auto. *)
-  (*     Qed. *)
-
-  (*   End WithSubstitution. *)
-  (*   (* #[global] Opaque wp. *) *)
-  (*   (* #[global] Opaque wlp. *) *)
-
-  (*   Lemma intro_wp_step' {Θ} {stepΘ : Step Θ} {lkStepΘ : LkStep Θ} *)
-  (*     {w α} (P : Pred w) (Q : Pred (w ، α)) (t : Ty) : *)
-  (*     (subst P step ⊢ₚ lift t =ₚ @oty.evar _ α world.in_zero ->ₚ Q) -> *)
-  (*     (P ⊢ₚ wp (step (Θ := Θ)) Q). *)
-  (*   Proof. *)
-  (*     pred_unfold. intros H ι HP. set (ι1 := env.snoc ι α t). exists ι1. *)
-  (*     specialize (H ι1). rewrite inst_step in H |- *; cbn in *. intuition. *)
-  (*   Qed. *)
-
-  (*   (* Better for iris proof mode. *) *)
-  (*   Lemma intro_wp_step {Θ} {stepΘ : Step Θ} {lkStepΘ : LkStep Θ} *)
-  (*     t {w α} (Q : Pred (w ، α)) : *)
-  (*     wlp step (lift t =ₚ oty.evar world.in_zero ->ₚ Q) ⊢ₚ wp (step (Θ := Θ)) Q. *)
-  (*   Proof. apply (intro_wp_step' t). now rewrite subst_wlp. Qed. *)
-
-  (*   (* Lemma wp_split  {Θ : SUB} [w0 w1] (θ : Θ w0 w1) P : *) *)
-  (*   (*   wp θ ⊤ₚ /\ₚ wlp θ P ⊢ₚ wp θ P. *) *)
-  (*   (* Proof. now rewrite and_wp_l, subst_wlp, and_true_l. Qed. *) *)
-
-  (*   Lemma wp_hmap `{LkHMap Θ1 Θ2} [w0 w1] (θ : Θ1 w0 w1) P : *)
-  (*     wp (hmap θ) P ⊣⊢ₚ wp θ P. *)
-  (*   Proof. *)
-  (*     constructor. intros ι0; cbn. apply ex_iff_morphism. *)
-  (*     intro ι1. now rewrite inst_hmap. *)
-  (*   Qed. *)
-
-  (*   Lemma wlp_hmap `{LkHMap Θ1 Θ2} [w0 w1] (θ : Θ1 w0 w1) P : *)
-  (*     wlp (hmap θ) P ⊣⊢ₚ wlp θ P. *)
-  (*   Proof. *)
-  (*     constructor. intros ι0; cbn. apply all_iff_morphism. *)
-  (*     intro ι1. now rewrite inst_hmap. *)
-  (*   Qed. *)
-
-  (* End Sub. *)
-
-  (* Definition PBox {Θ} : ⊧ Box Θ Pred ⇢ Pred := *)
-  (*   fun w Q => (∀ₚ w' (θ : Θ w w'), Sub.wlp θ (Q w' θ))%P. *)
-  (* Notation "◼ Q" := (PBox Q%B) (at level 9, right associativity, format "◼ Q"). *)
-
-  (* Section InstPred. *)
-  (*   Import iris.bi.derived_laws iris.bi.interface. *)
-
-  (*   (* A type class for things that can be interpreted as a predicate. *) *)
-  (*   Class InstPred (A : OType) := *)
-  (*     instpred : ⊧ A ⇢ Pred. *)
-  (*   #[global] Arguments instpred {_ _ _}. *)
-
-  (*   (* #[export] Instance instpred_option {A} `{ipA : InstPred A} : *) *)
-  (*   (*   InstPred (Option A) := *) *)
-  (*   (*   fun w o => wp_option o instpred. *) *)
-  (*   #[export] Instance instpred_list {A} `{ipA : InstPred A} : *)
-  (*     InstPred (List A) := *)
-  (*     fun w => *)
-  (*       fix ip xs {struct xs} := *)
-  (*       match xs with *)
-  (*       | nil       => ⊤ₚ *)
-  (*       | cons y ys => instpred y /\ₚ ip ys *)
-  (*       end%P. *)
-  (*   #[local] Instance instpred_prod_ty : InstPred (OTy * OTy) := *)
-  (*     fun w '(t1,t2) => eqₚ t1 t2. *)
-  (*   #[export] Instance instpred_unit : InstPred Unit := *)
-  (*     fun w _ => ⊤ₚ%P. *)
-  (*   #[global] Arguments instpred_unit [w] _ /. *)
-
-  (*   Lemma instpred_list_app {A} `{ipA : InstPred A} [w] (xs ys : List A w) : *)
-  (*     instpred (xs ++ ys) ⊣⊢ₚ instpred xs /\ₚ instpred ys. *)
-  (*   Proof. *)
-  (*     induction xs; cbn. *)
-  (*     - now rewrite and_true_l. *)
-  (*     - rewrite -bi.and_assoc. now apply bi.and_proper. *)
-  (*   Qed. *)
-
-  (*   Class InstPredSubst A {ipA : InstPred A} {subA : Subst A} := *)
-  (*     instpred_subst [Θ : SUB] {w0 w1} (θ : Θ w0 w1) (a : A w0) : *)
-  (*       instpred (subst a θ) ⊣⊢ₚ subst (instpred a) θ. *)
-  (*   #[global] Arguments InstPredSubst _ {_ _}. *)
-
-  (*   #[export] Instance instpred_subst_list `{InstPredSubst A} : *)
-  (*     InstPredSubst (List A). *)
-  (*   Proof. *)
-  (*     intros Θ w0 w1 θ xs. unfold subst, subst_list. *)
-  (*     induction xs; cbn; [easy|]. now rewrite instpred_subst IHxs. *)
-  (*   Qed. *)
-
-  (*   #[local] Instance instpred_subst_prod_ty : InstPredSubst (OTy * OTy). *)
-  (*   Proof. intros Θ w0 w1 θ [τ1 τ2]; cbn. now rewrite subst_eq. Qed. *)
-
-  (* End InstPred. *)
-
-  (* Lemma pno_cycle {w} (t1 t2 : OTy w) (Hsub : oty.OTy_subterm t1 t2) : *)
-  (*   t1 =ₚ t2 ⊢ₚ ⊥ₚ. *)
-  (* Proof. *)
-  (*   constructor. intros ι Heq. apply (inst_subterm ι) in Hsub. *)
-  (*   rewrite <- Heq in Hsub. now apply ty.no_cycle in Hsub. *)
-  (* Qed. *)
-
-  (* Lemma eqₚ_insert {w} (G1 G2 : OEnv w) (x : string) (t1 t2 : OTy w) : *)
-  (*   G1 =ₚ G2 /\ₚ t1 =ₚ t2 ⊢ₚ *)
-  (*   insert (M := OEnv w) x t1 G1 =ₚ insert (M := OEnv w) x t2 G2. *)
-  (* Proof. pred_unfold. intros []. now f_equal. Qed. *)
-
-  (* Lemma eq_func {w} (s1 s2 t1 t2 : OTy w) : *)
-  (*   oty.func s1 s2 =ₚ oty.func t1 t2 ⊣⊢ₚ (s1 =ₚ t1) /\ₚ (s2 =ₚ t2). *)
-  (* Proof. now rewrite peq_ty_noconfusion. Qed. *)
-
-  (* #[export] Instance params_tpb : Params (@TPB) 1 := {}. *)
-  (* #[export] Instance params_ifte : Params (@oexp.ifte) 1 := {}. *)
-  (* #[export] Instance params_eqₚ : Params (@eqₚ) 4 := {}. *)
-  (* #[export] Instance params_subst : Params (@subst) 4 := {}. *)
-
-  (* Section PBoxModality. *)
-  (*   Import iris.proofmode.tactics. *)
-
-  (*   #[export] Instance elimpbox `{LkRefl Θ} (p : bool) *)
-  (*     {w} (P : ◻Pred w) (Q : Pred w) : *)
-  (*     ElimModal True p true ◼P (P w refl) Q Q. *)
-  (*   Proof. *)
-  (*     intros _. unfold PBox. cbn. iIntros "[#H1 H2]". iApply "H2". *)
-  (*     destruct p; cbn; iSpecialize ("H1" $! w (refl (Refl := reflΘ))); *)
-  (*       now erewrite Sub.wlp_refl. *)
-  (*   Qed. *)
-
-  (*   Lemma subst_pbox `{LkTrans Θ} [w] (Q : ◻Pred w) [w1] (θ1 : Θ w w1) : *)
-  (*     (◼Q)[θ1] ⊢ₚ ◼(Q[θ1]). *)
-  (*   Proof. *)
-  (*     constructor; intros ι1 HQ w2 θ2 ι2 <-. *)
-  (*     apply HQ. now rewrite inst_trans. *)
-  (*   Qed. *)
-
-  (* End PBoxModality. *)
-
-  (* Section IntoSubst. *)
-
-  (*   Context {Θ : SUB}. *)
-
-  (*   Class IntoSubst `{Inst T A, Subst T} *)
-  (*     [w0 w1] (θ : Θ w0 w1) (x : T w0) (y : T w1) : Prop := *)
-  (*     into_subst : forall ι : Assignment w1, inst (subst x θ) ι = inst y ι. *)
-
-  (*   #[export] Instance into_subst_default `{Inst T A, Subst T} *)
-  (*     [w0 w1] (θ : Θ w0 w1) (t : T w0) : IntoSubst θ t (subst t θ) | 10. *)
-  (*   Proof. easy. Qed. *)
-
-  (*   (* #[export] Instance into_subst_subst `{LkTrans Θ, InstSubst T A} *) *)
-  (*   (*   [w0 w1 w2] (θ1 : Θ w0 w1) (θ2 : Θ w1 w2) (t : T w0) : *) *)
-  (*   (*   IntoSubst θ2 (subst t θ1) (subst t (trans θ1 θ2)) | 0. *) *)
-  (*   (* Proof. intros ι. now rewrite !inst_subst, inst_trans. Qed. *) *)
-
-  (*   #[export] Instance into_subst_lift {T A} {instTA : Inst T A} {liftTA : Lift T A} *)
-  (*     {subT : Subst T} {instLiftTA : InstLift T A} {instSubTA : InstSubst T A} *)
-  (*     [w0 w1] (θ : Θ w0 w1) (a : A) : *)
-  (*     IntoSubst θ (lift a) (lift a) | 0. *)
-  (*   Proof. intros ι. now rewrite inst_subst, !inst_lift. Qed. *)
-
-  (*   #[export] Instance into_subst_insert *)
-  (*     [w0 w1] (θ : Θ w0 w1) (G0 : OEnv w0) x (τ0 : OTy w0) G1 τ1 *)
-  (*     (HG : IntoSubst θ G0 G1) (Hτ : IntoSubst θ τ0 τ1) : *)
-  (*     IntoSubst θ (G0 ,, x ∷ τ0) (G1 ,, x ∷ τ1) | 0. *)
-  (*   Proof. *)
-  (*     intros ι1. specialize (HG ι1). specialize (Hτ ι1). *)
-  (*     change_no_check (@gmap.gmap string _ _ (OTy ?w)) with (OEnv w). *)
-  (*     rewrite subst_insert, !inst_insert. now f_equal. *)
-  (*   Qed. *)
-
-  (* End IntoSubst. *)
-
-  (* Section WlpModality. *)
-
-  (*   Import iris.proofmode.tactics. *)
-
-  (*   Context {Θ : SUB} [w0 w1] (θ : Θ w0 w1). *)
-
-  (*   Class IntoWlp (P : Pred w0) (Q : Pred w1) := *)
-  (*     into_wlp : P ⊢ Sub.wlp θ Q. *)
-
-  (*   #[export] Instance into_wlp_default (P : Pred w0) : *)
-  (*     IntoWlp P (subst P θ) | 10. *)
-  (*   Proof. unfold IntoWlp. now apply Sub.entails_wlp. Qed. *)
-
-  (*   Definition modality_wlp_mixin : *)
-  (*     modality_mixin (Sub.wlp θ) *)
-  (*       (MIEnvTransform IntoWlp) *)
-  (*       (MIEnvTransform IntoWlp). *)
-  (*   Proof. firstorder. Qed. *)
-
-  (*   Definition modality_wlp : modality bi_pred bi_pred := *)
-  (*     Modality _ (modality_wlp_mixin). *)
-
-  (*   #[export] Instance from_modal_wlp P : *)
-  (*     FromModal True modality_wlp (Sub.wlp θ P) (Sub.wlp θ P) P. *)
-  (*   Proof. firstorder. Qed. *)
-
-  (*   #[export] Instance into_wlp_pbox `{LkTrans Θ} (P : ◻Pred w0) : *)
-  (*     IntoWlp ◼P ◼(fun _ θ2 => P _ (θ ⊙ θ2)) | 0. *)
-  (*   Proof. unfold IntoWlp. iIntros "H !>". now rewrite subst_pbox. Qed. *)
-
-  (*   #[export] Instance into_wlp_tpb (G1 : OEnv w0) (e : Exp) (τ1 : OTy w0) *)
-  (*     (ee1 : OExp w0) G2 τ2 ee2 (HG : IntoSubst θ G1 G2) *)
-  (*     (Hτ : IntoSubst θ τ1 τ2) (Hee : IntoSubst θ ee1 ee2) : *)
-  (*     IntoWlp (TPB G1 e τ1 ee1) (TPB G2 e τ2 ee2) | 0. *)
-  (*   Proof. *)
-  (*     constructor. intros ι0 HT ι1 <-. pred_unfold. *)
-  (*     specialize (HG ι1). specialize (Hτ ι1). specialize (Hee ι1). *)
-  (*     rewrite !inst_subst in HG, Hτ, Hee. congruence. *)
-  (*   Qed. *)
-
-  (*   #[export] Instance into_wlp_eqp `{InstSubst T A} *)
-  (*     (x1 x2 : T w0) (y1 y2 : T w1) (Hxy1 : IntoSubst θ x1 y1) (Hxy2 :IntoSubst θ x2 y2) : *)
-  (*     IntoWlp (eqₚ x1 x2) (eqₚ y1 y2) | 0. *)
-  (*   Proof. *)
-  (*     constructor. pred_unfold. intros ι0 Heq ι1 ?Heq; cbn. *)
-  (*     specialize (Hxy1 ι1). specialize (Hxy2 ι1). *)
-  (*     rewrite !inst_subst in Hxy1, Hxy2. congruence. *)
-  (*   Qed. *)
-
-  (*   #[export] Instance into_wlp_wlp (P : Pred w1) : *)
-  (*     IntoWlp (Sub.wlp θ P) P | 0. *)
-  (*   Proof. unfold IntoWlp. reflexivity. Qed. *)
-
-  (* End WlpModality. *)
-
-  (* #[global] Arguments IntoWlp {Θ} [w0 w1] θ P Q. *)
-  (* #[global] Arguments into_wlp {Θ} [w0 w1] θ P Q {_}. *)
-  (* #[global] Hint Mode IntoWlp + + + + - - : typeclass_instances. *)
-
-  (* Import (hints) Par. *)
-
-  (* Create HintDb predsimpl. *)
-  (* #[export] Hint Rewrite (@subst_eq OEnv _ _ _ _) (@subst_eq OTy _ _ _ _) *)
-  (*   (@subst_refl OEnv _ _) (@subst_refl OTy _ _) (@subst_trans OEnv _ _) *)
-  (*   (@subst_trans OTy _ _) @Sub.wlp_refl @Sub.wlp_trans @Sub.wlp_true *)
-  (*   @Sub.wp_false @Sub.wp_refl @Sub.wp_trans @and_false_l @and_false_r *)
-  (*   @and_true_l @and_true_r @eq_func @eqₚ_refl @impl_and @impl_false_l *)
-  (*   @impl_true_l @impl_true_r @lk_refl @lk_step @lk_trans @subst_and @subst_false *)
-  (*   @subst_pred_refl @subst_pred_trans @subst_tpb @subst_true @trans_refl_r *)
-  (*   : predsimpl. *)
-  (* Ltac predsimpl := *)
-  (*   repeat *)
-  (*     (try (progress cbn); unfold _4; *)
-  (*      change_no_check (@gmap.gmap string _ _ (OTy ?w)) with (OEnv w) in *; *)
-  (*      repeat *)
-  (*        match goal with *)
-  (*        | |- Sub.wp ?θ _ ⊣⊢ₚ Sub.wp ?θ _ => apply Sub.proper_wp_bientails *)
-  (*        | |- Sub.wlp ?θ _ ⊣⊢ₚ Sub.wlp ?θ _ => apply Sub.proper_wlp_bientails *)
-  (*        end; *)
-  (*      try easy; repeat rewrite_db predsimpl; auto 1 with typeclass_instances; *)
-  (*      repeat *)
-  (*        match goal with *)
-  (*        | |- context[@subst ?A ?I ?Θ ?w0 ?x ?w1 ?θ] => *)
-  (*            is_var x; generalize (@subst A I Θ w0 x w1 θ); clear x; intros x; *)
-  (*            try (clear w0 θ) *)
-  (*        | |- context[@lk ?Θ (?w0 ، ?α) ?w1 ?θ ?α world.in_zero] => *)
-  (*            is_var θ; *)
-  (*            generalize (@lk Θ (w0 ، α) w1 θ α world.in_zero); *)
-  (*            clear θ w0; intros ?t *)
-  (*        end). *)
 
 End Pred.
